added spec, linked to kyber768, proof for one module

proofs/fstar/extraction-edited/Libcrux.Kem.Kyber.Kyber768.fst
@@ -62,36 +62,21 @@ let v_CPA_PKE_CIPHERTEXT_SIZE_768_: usize = v_C1_SIZE_768_ +! v_C2_SIZE_768_
 let v_IMPLICIT_REJECTION_HASH_INPUT_SIZE: usize =
   Libcrux.Kem.Kyber.Constants.v_SHARED_SECRET_SIZE +! v_CPA_PKE_CIPHERTEXT_SIZE_768_
 
-unfold
-let t_Kyber768Ciphertext = Libcrux.Kem.Kyber.Types.t_KyberCiphertext (sz 1088)
-
-unfold
-let t_Kyber768PrivateKey = Libcrux.Kem.Kyber.Types.t_KyberPrivateKey (sz 2400)
-
-unfold
-let t_Kyber768PublicKey = Libcrux.Kem.Kyber.Types.t_KyberPublicKey (sz 1184)
-
 let decapsulate_768_
       (secret_key: Libcrux.Kem.Kyber.Types.t_KyberPrivateKey (sz 2400))
-      (ciphertext: Libcrux.Kem.Kyber.Types.t_KyberCiphertext (sz 1088))
-    : t_Array u8 (sz 32) =
+      (ciphertext: Libcrux.Kem.Kyber.Types.t_KyberCiphertext (sz 1088)) =
   Libcrux.Kem.Kyber.decapsulate (sz 3) (sz 2400) (sz 1152) (sz 1184) (sz 1088) (sz 1152) (sz 960)
     (sz 128) (sz 10) (sz 4) (sz 320) (sz 2) (sz 128) (sz 2) (sz 128) (sz 1120) secret_key ciphertext
 
 
 let encapsulate_768_
       (public_key: Libcrux.Kem.Kyber.Types.t_KyberPublicKey (sz 1184))
-      (randomness: t_Array u8 (sz 32))
-    : Core.Result.t_Result
-      (Libcrux.Kem.Kyber.Types.t_KyberCiphertext (sz 1088) & t_Array u8 (sz 32))
-      Libcrux.Kem.Kyber.Types.t_Error =
+      (randomness: t_Array u8 (sz 32)) =
   Libcrux.Kem.Kyber.encapsulate (sz 3) (sz 1088) (sz 1184) (sz 1152) (sz 960) (sz 128) (sz 10)
     (sz 4) (sz 320) (sz 2) (sz 128) (sz 2) (sz 128) public_key randomness
 
-let generate_key_pair_768_ (randomness: t_Array u8 (sz 64))
-    : Core.Result.t_Result (Libcrux.Kem.Kyber.Types.t_KyberKeyPair (sz 2400) (sz 1184))
-      Libcrux.Kem.Kyber.Types.t_Error =
-  Libcrux.Kem.Kyber.generate_keypair (sz 3)
+let generate_key_pair_768_ (randomness: t_Array u8 (sz 64)) =
+  Libcrux.Kem.Kyber.generate_keypair #Spec.Kyber.kyber768_params (sz 3)
     (sz 1152)
     (sz 2400)
     (sz 1184)
