proofs/fstar/extraction-edited/Libcrux.Kem.Kyber.fsti
@@ -3,33 +3,62 @@ module Libcrux.Kem.Kyber
 open Core
 open FStar.Mul
 
-
-// KB: Note that the 32 in the pre-condition  below is the size of the implicit_rejection_value.
-//     Should we have a constant in Constants with this size a well?
-
 val decapsulate
       (v_K v_SECRET_KEY_SIZE v_CPA_SECRET_KEY_SIZE v_PUBLIC_KEY_SIZE v_CIPHERTEXT_SIZE v_T_AS_NTT_ENCODED_SIZE v_C1_SIZE v_C2_SIZE v_VECTOR_U_COMPRESSION_FACTOR v_VECTOR_V_COMPRESSION_FACTOR v_C1_BLOCK_SIZE v_ETA1 v_ETA1_RANDOMNESS_SIZE v_ETA2 v_ETA2_RANDOMNESS_SIZE v_IMPLICIT_REJECTION_HASH_INPUT_SIZE:
           usize)
       (secret_key: Libcrux.Kem.Kyber.Types.t_KyberPrivateKey v_SECRET_KEY_SIZE)
       (ciphertext: Libcrux.Kem.Kyber.Types.t_KyberCiphertext v_CIPHERTEXT_SIZE)
     : Pure (t_Array u8 (sz 32))
-    (requires (Libcrux.Kem.Kyber.Constants.v_SHARED_SECRET_SIZE <. v_IMPLICIT_REJECTION_HASH_INPUT_SIZE /\
-               v v_SECRET_KEY_SIZE == v v_CPA_SECRET_KEY_SIZE + v v_PUBLIC_KEY_SIZE + v Libcrux.Kem.Kyber.Constants.v_H_DIGEST_SIZE + 32))
-    (ensures (fun res -> True))
+    (requires (let p = let open Spec.Kyber in {v_RANK = v_K; v_ETA1; v_ETA2; v_VECTOR_U_COMPRESSION_FACTOR; v_VECTOR_V_COMPRESSION_FACTOR} in
+                Spec.Kyber.valid_params p /\
+                v_IMPLICIT_REJECTION_HASH_INPUT_SIZE == Spec.Kyber.v_IMPLICIT_REJECTION_HASH_INPUT_SIZE p /\
+                v_CPA_SECRET_KEY_SIZE == Spec.Kyber.v_CPA_PKE_SECRET_KEY_SIZE p /\
+                v_SECRET_KEY_SIZE == Spec.Kyber.v_SECRET_KEY_SIZE p /\
+                v_PUBLIC_KEY_SIZE == Spec.Kyber.v_CPA_PKE_PUBLIC_KEY_SIZE p /\
+                v_CIPHERTEXT_SIZE == Spec.Kyber.v_CPA_PKE_CIPHERTEXT_SIZE p
+               ))
+    (ensures (fun res ->
+                let open Spec.Kyber in
+                let p = {v_RANK = v_K; v_ETA1; v_ETA2; v_VECTOR_U_COMPRESSION_FACTOR; v_VECTOR_V_COMPRESSION_FACTOR} in
+                res == Spec.Kyber.ind_cca_decapsulate p secret_key.f_value ciphertext.f_value))
 
 val encapsulate
       (v_K v_CIPHERTEXT_SIZE v_PUBLIC_KEY_SIZE v_T_AS_NTT_ENCODED_SIZE v_C1_SIZE v_C2_SIZE v_VECTOR_U_COMPRESSION_FACTOR v_VECTOR_V_COMPRESSION_FACTOR v_VECTOR_U_BLOCK_LEN v_ETA1 v_ETA1_RANDOMNESS_SIZE v_ETA2 v_ETA2_RANDOMNESS_SIZE:
           usize)
       (public_key: Libcrux.Kem.Kyber.Types.t_KyberPublicKey v_PUBLIC_KEY_SIZE)
       (randomness: t_Array u8 (sz 32))
-    : Core.Result.t_Result
-      (Libcrux.Kem.Kyber.Types.t_KyberCiphertext v_CIPHERTEXT_SIZE & t_Array u8 (sz 32))
-      Libcrux.Kem.Kyber.Types.t_Error
+    : Pure (Core.Result.t_Result
+           (Libcrux.Kem.Kyber.Types.t_KyberCiphertext v_CIPHERTEXT_SIZE & t_Array u8 (sz 32))
+            Libcrux.Kem.Kyber.Types.t_Error)
+      (requires (
+                let p = let open Spec.Kyber in {v_RANK = v_K; v_ETA1; v_ETA2; v_VECTOR_U_COMPRESSION_FACTOR; v_VECTOR_V_COMPRESSION_FACTOR} in
+                Spec.Kyber.valid_params p /\
+                v_PUBLIC_KEY_SIZE == Spec.Kyber.v_CPA_PKE_PUBLIC_KEY_SIZE p /\
+                v_CIPHERTEXT_SIZE == Spec.Kyber.v_CPA_PKE_CIPHERTEXT_SIZE p
+                ))
 
-val generate_keypair
+      (ensures (fun res ->
+                let open Spec.Kyber in
+                let p = {v_RANK = v_K; v_ETA1; v_ETA2; v_VECTOR_U_COMPRESSION_FACTOR; v_VECTOR_V_COMPRESSION_FACTOR} in
+                let spec_result = Spec.Kyber.ind_cca_encapsulate p public_key.f_value randomness in
+                match res with 
+                | Core.Result.Result_Ok (cip,ss) -> spec_result == Ok(cip.f_value,ss)
+                | Core.Result.Result_Err e -> spec_result = Err Error_RejectionSampling))
+
+val generate_keypair (#p:Spec.Kyber.params)
       (v_K v_CPA_PRIVATE_KEY_SIZE v_PRIVATE_KEY_SIZE v_PUBLIC_KEY_SIZE v_BYTES_PER_RING_ELEMENT v_ETA1 v_ETA1_RANDOMNESS_SIZE:
           usize)
       (randomness: t_Array u8 (sz 64))
-    : Core.Result.t_Result
-      (Libcrux.Kem.Kyber.Types.t_KyberKeyPair v_PRIVATE_KEY_SIZE v_PUBLIC_KEY_SIZE)
-      Libcrux.Kem.Kyber.Types.t_Error
+    : Pure (Core.Result.t_Result
+           (Libcrux.Kem.Kyber.Types.t_KyberKeyPair v_PRIVATE_KEY_SIZE v_PUBLIC_KEY_SIZE)
+           Libcrux.Kem.Kyber.Types.t_Error)
+      (requires (v_K == p.v_RANK /\ v_ETA1 == p.v_ETA1 /\
+                v_PUBLIC_KEY_SIZE == Spec.Kyber.v_CPA_PKE_PUBLIC_KEY_SIZE p /\
+                v_PRIVATE_KEY_SIZE == Spec.Kyber.v_SECRET_KEY_SIZE p
+                ))
+
+      (ensures (fun res -> 
+                let spec_result = Spec.Kyber.ind_cca_generate_keypair p randomness in
+                match res with 
+                | Core.Result.Result_Ok (kp) -> spec_result == Spec.Kyber.Ok(kp.Libcrux.Kem.Kyber.Types.f_sk.f_value,kp.Libcrux.Kem.Kyber.Types.f_pk.f_value)
+                | Core.Result.Result_Err e -> spec_result = Spec.Kyber.Err Spec.Kyber.Error_RejectionSampling))
