proofs/fstar/extraction-edited/Libcrux.Kem.Kyber.Kyber768.fsti
@@ -1,0 +1,36 @@
+module Libcrux.Kem.Kyber.Kyber768
+#set-options "--fuel 0 --ifuel 1 --z3rlimit 15"
+open Core
+open FStar.Mul
+
+unfold
+let t_Kyber768Ciphertext = Libcrux.Kem.Kyber.Types.t_KyberCiphertext (sz 1088)
+
+unfold
+let t_Kyber768PrivateKey = Libcrux.Kem.Kyber.Types.t_KyberPrivateKey (sz 2400)
+
+unfold
+let t_Kyber768PublicKey = Libcrux.Kem.Kyber.Types.t_KyberPublicKey (sz 1184)
+
+val decapsulate_768_
+      (secret_key: Libcrux.Kem.Kyber.Types.t_KyberPrivateKey (sz 2400))
+      (ciphertext: Libcrux.Kem.Kyber.Types.t_KyberCiphertext (sz 1088))
+      : Pure (t_Array u8 (sz 32))
+      (requires True)
+      (ensures (fun res -> res == Spec.Kyber.kyber768_decapsulate secret_key.f_value ciphertext.f_value))
+
+val encapsulate_768_
+      (public_key: Libcrux.Kem.Kyber.Types.t_KyberPublicKey (sz 1184))
+      (randomness: t_Array u8 (sz 32))
+    : Pure (Core.Result.t_Result
+           (Libcrux.Kem.Kyber.Types.t_KyberCiphertext (sz 1088) & t_Array u8 (sz 32))
+            Libcrux.Kem.Kyber.Types.t_Error)
+      (requires True)
+      (ensures (fun res -> True))
+
+val generate_key_pair_768_ (randomness: t_Array u8 (sz 64))
+    : Pure (Core.Result.t_Result (Libcrux.Kem.Kyber.Types.t_KyberKeyPair (sz 2400) (sz 1184))
+            Libcrux.Kem.Kyber.Types.t_Error )
+      (requires (True))
+      (ensures (fun res -> True))
+
